Started into stack assembling, got one case done

12UnstructuredMemory/UnstructuredMemory.thy
@@ -1,5 +1,5 @@
 theory UnstructuredMemory
-  imports "../08FlatCode/ByteCode"
+  imports "../08FlatCode/CodeFlattening"
 begin
 
 datatype unstr_state = 
@@ -70,5 +70,211 @@ next
     by (induction cd "US h hp e ep vs (Suc (Suc vp)) sh sp (Suc pc)" \<Sigma>'' rule: evalu.induct) 
        simp_all
 qed
+
+definition restructurable_heap :: "(nat \<Rightarrow> nat) \<Rightarrow> nat \<Rightarrow> nat \<Rightarrow> nat \<Rightarrow> bool" where
+  "restructurable_heap h hp ep lcd = (3 dvd hp \<and> (\<forall>x < hp. 3 dvd x \<longrightarrow> h x \<noteq> 0 \<longrightarrow> 
+    (even (h (Suc x)) \<and> (h (Suc x)) \<le> ep \<and> h (Suc (Suc x)) \<noteq> 0 \<and> h (Suc (Suc x)) \<le> lcd)))"
+
+definition restructurable_env :: "(nat \<Rightarrow> nat) \<Rightarrow> nat \<Rightarrow> nat \<Rightarrow> bool" where
+  "restructurable_env e ep hp = (even ep \<and>
+    (\<forall>x < ep. if even x then 3 dvd e x \<and> e x < hp else even (e x) \<and> e x \<le> ep))"
+
+definition restructurable_vals :: "(nat \<Rightarrow> nat) \<Rightarrow> nat \<Rightarrow> nat \<Rightarrow> bool" where
+  "restructurable_vals vs vp hp = (\<forall>x < vp. 3 dvd vs x \<and> vs x < hp)"
+
+definition restructurable_stack :: "(nat \<Rightarrow> nat) \<Rightarrow> nat \<Rightarrow> nat \<Rightarrow> nat \<Rightarrow> bool" where
+  "restructurable_stack sh sp ep lcd = 
+    (\<forall>x < sp. if odd x then sh x \<noteq> 0 \<and> sh x \<le> lcd else even (sh x) \<and> sh x \<le> ep)"
+
+primrec restructurable :: "unstr_state \<Rightarrow> byte_code list \<Rightarrow> bool" where
+  "restructurable (US h hp e ep vs vp sh sp pc) cd = (pc \<le> length cd \<and> 
+    length cd \<noteq> 0 \<and> orderly cd 0 \<and> return_terminated cd \<and> restructurable_heap h hp ep (length cd) \<and> 
+      restructurable_env e ep hp \<and> restructurable_vals vs vp hp \<and> 
+        restructurable_stack sh sp ep (length cd) \<and> (if pc = 0 then sp = 0 else odd sp))"
+
+lemma [simp]: "odd (x::nat) \<Longrightarrow> 0 < x"
+  by (cases x) simp_all
+
+lemma [simp]: "return_terminated cd \<Longrightarrow> cd ! 0 \<noteq> BLookup x"
+  by (induction cd) auto
+
+lemma [simp]: "return_terminated cd \<Longrightarrow> cd ! 0 \<noteq> BPushCon k"
+  by (induction cd) auto
+
+lemma [simp]: "return_terminated cd \<Longrightarrow> cd ! 0 \<noteq> BPushLam pc"
+  by (induction cd) auto
+
+lemma [simp]: "return_terminated cd \<Longrightarrow> cd ! 0 \<noteq> BApply"
+  by (induction cd) auto
+
+lemma [dest]: "x \<noteq> y \<Longrightarrow> x < Suc y \<Longrightarrow> x < y"
+  by presburger
+
+lemma [dest]: "x \<noteq> y \<Longrightarrow> x \<noteq> Suc y \<Longrightarrow> x < Suc (Suc y) \<Longrightarrow> x < y"
+  by presburger
+
+lemma [simp]: "3 dvd x \<Longrightarrow> 3 dvd Suc x = False"
+  by presburger
+
+lemma [simp]: "3 dvd x \<Longrightarrow> 3 dvd Suc (Suc x) = False"
+  by presburger
+
+lemma [elim]: "restructurable_env e ep hp \<Longrightarrow> even ep"
+  by (simp add: restructurable_env_def)
+
+lemma [elim]: "restructurable_heap h hp ep lcd \<Longrightarrow> 3 dvd hp"
+  by (simp add: restructurable_heap_def)
+
+lemma [simp]: "restructurable_heap h hp ep lcd \<Longrightarrow> 
+    restructurable_heap (h(hp := 0, Suc hp := k, Suc (Suc hp) := 0)) (3 + hp) ep lcd"
+  by (auto simp add: restructurable_heap_def)
+
+lemma [simp]: "restructurable_heap h hp ep lcd \<Longrightarrow> lcd \<noteq> 0 \<Longrightarrow>
+  restructurable_heap (h(hp := Suc 0, Suc hp := k, Suc (Suc hp) := pc)) (3 + hp) ep lcd = 
+    (even k \<and> k \<le> ep \<and> pc \<noteq> 0 \<and> pc \<le> lcd)"
+proof
+  let ?f = "\<lambda>x. if x = Suc (Suc hp) then pc else (h(hp := Suc 0, Suc hp := k)) x"
+  let ?g = "\<lambda>x. if x = Suc hp then pc else (h(hp := Suc 0, Suc hp := k)) (Suc x)"
+  let ?h = "\<lambda>x. if x = hp then pc else (h(hp := Suc 0, Suc hp := k)) (Suc (Suc x))"
+  assume H: "restructurable_heap (h(hp := Suc 0, Suc hp := k, Suc (Suc hp) := pc)) (3 + hp) ep lcd"
+  moreover hence "\<And>x. x < 3 + hp \<Longrightarrow> 3 dvd x \<Longrightarrow> 0 < ?f x \<and> ?f x \<le> lcd \<Longrightarrow> 
+    even (?g x) \<and> ?g x \<le> ep \<and> 0 < ?h x \<and> ?h x \<le> lcd" by (simp add: restructurable_heap_def)
+  moreover from H have "3 dvd hp" by (simp add: restructurable_heap_def)
+  ultimately have "hp < 3 + hp \<Longrightarrow> 0 < ?f hp \<and> ?f hp \<le> lcd \<Longrightarrow> 
+    even (?g hp) \<and> ?g hp \<le> ep \<and> 0 < ?h hp \<and> ?h hp \<le> lcd" by blast
+  moreover assume "lcd \<noteq> 0"
+  ultimately show "even k \<and> k \<le> ep \<and> pc \<noteq> 0 \<and> pc \<le> lcd" by simp
+next
+  assume "restructurable_heap h hp ep lcd" and "even k \<and> k \<le> ep \<and> pc \<noteq> 0 \<and> pc \<le> lcd"
+  thus "restructurable_heap (h(hp := Suc 0, Suc hp := k, Suc (Suc hp) := pc)) (3 + hp) ep lcd" 
+    by (auto simp add: restructurable_heap_def)
+qed
+
+lemma [simp]: "restructurable_heap h hp ep lcd \<Longrightarrow> restructurable_heap h hp (Suc (Suc ep)) lcd"
+  by (auto simp add: restructurable_heap_def)
+
+lemma [simp]: "restructurable_env e ep hp \<Longrightarrow> restructurable_env e ep (3 + hp)"
+  by (auto simp add: restructurable_env_def)
+
+lemma [simp]: "restructurable_env e ep hp \<Longrightarrow> restructurable_vals vs (Suc (Suc vp)) hp \<Longrightarrow> 
+  restructurable_heap h hp ep lcd \<Longrightarrow> h (vs vp) = Suc x \<Longrightarrow>
+    restructurable_env (e(ep := vs (Suc vp), Suc ep := h (Suc (vs vp)))) (Suc (Suc ep)) hp"
+proof (unfold restructurable_env_def restructurable_vals_def restructurable_heap_def, 
+       rule, simp, rule, rule)
+  fix y 
+  assume "3 dvd hp \<and> (\<forall>x < hp. 3 dvd x \<longrightarrow> h x \<noteq> 0 \<longrightarrow> 
+    even (h (Suc x)) \<and> h (Suc x) \<le> ep \<and> h (Suc (Suc x)) \<noteq> 0 \<and> h (Suc (Suc x)) \<le> lcd)"
+     and "h (vs vp) = Suc x" and "\<forall>x < Suc (Suc vp). 3 dvd vs x \<and> vs x < hp"
+  hence "even (h (Suc (vs vp))) \<and> h (Suc (vs vp)) \<le> ep" by simp
+  moreover assume "even ep \<and> 
+    (\<forall>x < ep. if even x then 3 dvd e x \<and> e x < hp else even (e x) \<and> e x \<le> ep)"
+              and "y < Suc (Suc ep)" and "\<forall>x < Suc (Suc vp). 3 dvd vs x \<and> vs x < hp"
+  ultimately show "if even y
+        then 3 dvd (e(ep := vs (Suc vp), Suc ep := h (Suc (vs vp)))) y \<and> 
+          (e(ep := vs (Suc vp), Suc ep := h (Suc (vs vp)))) y < hp
+        else even ((e(ep := vs (Suc vp), Suc ep := h (Suc (vs vp)))) y) \<and>
+          (e(ep := vs (Suc vp), Suc ep := h (Suc (vs vp)))) y \<le> Suc (Suc ep)" by auto
+qed
+
+lemma [simp]: "restructurable_vals vs vp hp \<Longrightarrow> 
+    restructurable_vals (vs(vp := k)) (Suc vp) hp = (k < hp \<and> 3 dvd k)"
+  by (auto simp add: restructurable_vals_def)
+
+lemma [simp]: "restructurable_vals vs vp hp \<Longrightarrow> 
+    restructurable_vals (vs(vp := k)) (Suc vp) (3 + hp) = (k < 3 + hp \<and> 3 dvd k)"
+  by (auto simp add: restructurable_vals_def)
+
+lemma [elim]: "restructurable_vals vs (Suc (Suc vp)) hp \<Longrightarrow> restructurable_vals vs vp hp"
+  by (simp add: restructurable_vals_def)
+
+lemma [elim]: "restructurable_stack sh (Suc (Suc sp)) ep lcd \<Longrightarrow> restructurable_stack sh sp ep lcd"
+  by (simp add: restructurable_stack_def)
+
+lemma [simp]: "restructurable_stack sh 0 ep lcd"
+  by (simp add: restructurable_stack_def)
+
+lemma [simp]: "restructurable_stack sh (Suc (Suc sp)) ep lcd \<Longrightarrow> odd sp \<Longrightarrow> sh sp \<noteq> 0"
+  by (simp add: restructurable_stack_def)
+
+lemma [simp]: "restructurable_stack sh (Suc (Suc sp)) ep lcd \<Longrightarrow> odd sp \<Longrightarrow> sh sp \<le> lcd"
+  by (simp add: restructurable_stack_def)
+
+lemma [simp]: "restructurable_stack sh sp ep lcd \<Longrightarrow> odd sp \<Longrightarrow> pc \<noteq> 0 \<Longrightarrow> Suc pc \<le> lcd \<Longrightarrow> 
+  even ep \<Longrightarrow> 
+    restructurable_stack (sh(sp := pc, Suc sp := Suc (Suc ep))) (Suc (Suc sp)) (Suc (Suc ep)) lcd"
+  by (unfold restructurable_stack_def) auto
+
+lemma [simp]: "restructurable_stack sh sp ep lcd \<Longrightarrow> odd sp \<Longrightarrow> Suc pc \<le> lcd \<Longrightarrow> 
+  restructurable_env e ep hp \<Longrightarrow> return_terminated cd \<Longrightarrow> cd ! pc = BApply \<Longrightarrow> 
+    restructurable_stack (sh(sp := pc, Suc sp := Suc (Suc ep))) (Suc (Suc sp)) (Suc (Suc ep)) lcd"
+proof -
+  assume "return_terminated cd" and "cd ! pc = BApply"
+  hence "pc = 0 \<Longrightarrow> False" by simp
+  hence "pc \<noteq> 0" by auto
+  moreover assume "restructurable_env e ep hp"
+  moreover hence "even ep" by auto
+  moreover assume "restructurable_stack sh sp ep lcd" and "odd sp" and "Suc pc \<le> lcd"
+  ultimately show ?thesis by simp
+qed
+
+lemma [simp]: "restructurable_env e ep hp \<Longrightarrow> restructurable_stack sh sp ep lcd \<Longrightarrow> odd sp \<Longrightarrow> 
+    restructurable_stack (sh(sp - Suc 0 := Suc (Suc ep))) sp (Suc (Suc ep)) lcd"
+  by (unfold restructurable_stack_def) auto
+
+lemma [simp]: "h (vs vp) = Suc y \<Longrightarrow> restructurable_heap h hp ep lcd \<Longrightarrow> 
+    restructurable_vals vs (Suc (Suc vp)) hp \<Longrightarrow> 0 < h (Suc (Suc (vs vp)))"
+  by (simp add: restructurable_heap_def restructurable_vals_def)
+
+lemma [simp]: "h (vs vp) = Suc y \<Longrightarrow> restructurable_heap h hp ep lcd \<Longrightarrow> 
+    restructurable_vals vs (Suc (Suc vp)) hp \<Longrightarrow> h (Suc (Suc (vs vp))) \<le> lcd"
+  by (simp add: restructurable_heap_def restructurable_vals_def)
+
+lemma [elim]: "unstr_lookup e p x = Some y \<Longrightarrow> p \<le> ep \<Longrightarrow> even p \<Longrightarrow> restructurable_env e ep hp \<Longrightarrow> 
+    y < hp"
+proof (induction e p x rule: unstr_lookup.induct)
+  case (4 e p x)
+  moreover hence "even (e (Suc p)) \<and> e (Suc p) \<le> ep" by (simp add: restructurable_env_def)
+  ultimately show ?case by simp
+qed (auto simp add: restructurable_env_def)
+
+lemma [elim]: "unstr_lookup e p x = Some y \<Longrightarrow> p \<le> ep \<Longrightarrow> even p \<Longrightarrow> restructurable_env e ep hp \<Longrightarrow> 
+    3 dvd y"
+proof (induction e p x rule: unstr_lookup.induct) 
+  case (4 e p x)
+  moreover hence "even (e (Suc p)) \<and> e (Suc p) \<le> ep" by (simp add: restructurable_env_def)
+  ultimately show ?case by simp
+qed (auto simp add: restructurable_env_def)
+
+lemma [simp]: "odd sp \<Longrightarrow> restructurable_stack sh sp ep lcd \<Longrightarrow> even (sh (sp - Suc 0))" 
+  by (unfold restructurable_stack_def) auto
+
+lemma [simp]: "odd sp \<Longrightarrow> restructurable_stack sh sp ep lcd \<Longrightarrow> sh (sp - Suc 0) \<le> ep" 
+  by (unfold restructurable_stack_def) auto
+
+lemma [elim]: "unstr_lookup e (sh (sp - Suc 0)) x = Some y \<Longrightarrow> restructurable_stack sh sp ep lcd \<Longrightarrow> 
+  restructurable_env e ep hp \<Longrightarrow> odd sp \<Longrightarrow> y < hp"
+proof -
+  assume "odd sp" and "restructurable_stack sh sp ep lcd"  
+  hence "even (sh (sp - Suc 0))" and "sh (sp - Suc 0) \<le> ep" by auto
+  moreover assume "unstr_lookup e (sh (sp - Suc 0)) x = Some y" and "restructurable_env e ep hp"
+  ultimately show "y < hp" by auto
+qed
+
+lemma [elim]: "unstr_lookup e (sh (sp - Suc 0)) x = Some y \<Longrightarrow> restructurable_stack sh sp ep lcd \<Longrightarrow> 
+    restructurable_env e ep hp \<Longrightarrow> odd sp \<Longrightarrow> 3 dvd y"
+proof -
+  assume "odd sp" and "restructurable_stack sh sp ep lcd"  
+  hence "sh (sp - Suc 0) \<le> ep \<and> even (sh (sp - Suc 0))" by (unfold restructurable_stack_def) auto
+  moreover assume "unstr_lookup e (sh (sp - Suc 0)) x = Some y" and "restructurable_env e ep hp"
+  ultimately show "3 dvd y" by auto
+qed
+
+lemma [simp]: "h (vs vp) = Suc x \<Longrightarrow> restructurable_heap h hp ep (length cd) \<Longrightarrow> 
+    restructurable_vals vs (Suc (Suc vp)) hp \<Longrightarrow> h (Suc (Suc (vs vp))) \<noteq> 0"
+  by simp
+
+lemma preserve_restructure [simp]: "cd \<tturnstile> \<Sigma>\<^sub>u \<leadsto>\<^sub>u \<Sigma>\<^sub>u' \<Longrightarrow> restructurable \<Sigma>\<^sub>u cd \<Longrightarrow> 
+    restructurable \<Sigma>\<^sub>u' cd"
+  by (induction \<Sigma>\<^sub>u \<Sigma>\<^sub>u' rule: evalu.induct) auto
 
 end
