13StackAssembly/AssembleStack.thy
@@ -4,8 +4,8 @@ begin
 
 primrec assemble_stack_len :: "byte_code \<Rightarrow> nat" where
   "assemble_stack_len (BLookup x) = 1"
-| "assemble_stack_len (BPushCon k) = 5"
-| "assemble_stack_len (BPushLam pc) = 1"
+| "assemble_stack_len (BPushCon k) = 6"
+| "assemble_stack_len (BPushLam pc) = 9"
 | "assemble_stack_len BApply = 1"
 | "assemble_stack_len BReturn = 1"
 | "assemble_stack_len BJump = 1"
@@ -13,22 +13,28 @@ primrec assemble_stack_len :: "byte_code \<Rightarrow> nat" where
 primrec assemble_stack_op :: "(nat \<Rightarrow> nat) \<Rightarrow> byte_code \<Rightarrow> sassm_code list" where
   "assemble_stack_op mp (BLookup x) = [undefined]"
 | "assemble_stack_op mp (BPushCon k) = [
+    SAMov (MCon 0),
     SAPush Hp (Con 0), 
     SAPush Hp (Con k), 
     SAPush Hp (Con 0), 
     SAPush Vals Acc, 
-    SAMov Hp]"
-| "assemble_stack_op mp (BPushLam pc) = [undefined]"
+    SAMov (Mem Hp)]"
+| "assemble_stack_op mp (BPushLam pc) = [
+    SAMov (MCon 0),
+    SAPush Hp (Con (mp pc)), 
+    SAPush Hp Acc, 
+    SAPush Hp (Con 1),
+    SAGet Stk, 
+    SASub 1,
+    SAMov (Mem Stk),
+    SAPush Vals Acc, 
+    SAMov (Mem Hp)]"
 | "assemble_stack_op mp BApply = [undefined]"
 | "assemble_stack_op mp BReturn = [undefined]"
 | "assemble_stack_op mp BJump = [undefined]"
 
 (*   evu_lookup [simp]: "cd ! pc = BLookup x \<Longrightarrow> unstr_lookup e (sh (sp - 1)) x = Some y \<Longrightarrow>
     cd \<tturnstile> US h hp e ep vs vp sh sp (Suc pc) \<leadsto>\<^sub>u US h hp e ep (vs(vp := y)) (Suc vp) sh sp pc"
-| evu_pushlam [simp]: "cd ! pc = BPushLam pc' \<Longrightarrow> 
-    cd \<tturnstile> US h hp e ep vs vp sh sp (Suc pc) \<leadsto>\<^sub>u 
-      US (h(hp := 1, Suc hp := sh (sp - 1), Suc (Suc hp) := pc')) (3 + hp) e ep 
-        (vs(vp := hp)) (Suc vp) sh sp pc"
 | evu_apply [simp]: "cd ! pc = BApply \<Longrightarrow> h (vs vp) = Suc x \<Longrightarrow> 
     cd \<tturnstile> US h hp e ep vs (Suc (Suc vp)) sh sp (Suc pc) \<leadsto>\<^sub>u 
       US h hp (e(ep := vs (Suc vp), Suc ep := h (Suc (vs vp)))) (2 + ep) vs vp
@@ -47,7 +53,7 @@ abbreviation assemble_extend_map :: "(nat \<Rightarrow> nat) \<Rightarrow> nat \
 
 fun assembly_map :: "byte_code list \<Rightarrow> nat \<Rightarrow> nat" where
   "assembly_map [] x = x"
-| "assembly_map (op # cd) 0 = assemble_stack_len op - 1"
+| "assembly_map (op # cd) 0 = 0"
 | "assembly_map (op # cd) (Suc x) = assemble_stack_len op + assembly_map cd x"
 
 definition assemble_stack_code :: "byte_code list \<Rightarrow> sassm_code list" where
@@ -55,15 +61,14 @@ definition assemble_stack_code :: "byte_code list \<Rightarrow> sassm_code list"
 
 primrec assemble_state :: "(nat \<Rightarrow> nat) \<Rightarrow> unstr_state \<Rightarrow> sassm_state" where
   "assemble_state mp (US h hp e ep vs vp sh sp pc) = 
-    SAS (\<lambda>m. case m of Hp \<Rightarrow> h | Env \<Rightarrow> e | Vals \<Rightarrow> vs | Stk \<Rightarrow> sh) 
-      (\<lambda>m. case m of Hp \<Rightarrow> hp | Env \<Rightarrow> ep | Vals \<Rightarrow> vp | Stk \<Rightarrow> sp) (SOME x. True) (mp pc)"
+    SAS (case_memory h e vs sh) (case_memory hp ep vp sp) 0 (mp pc)"
 
-lemma [simp]: "assemble_stack_len op = length (assemble_stack_op mp op)"
+lemma [simp]: "length (assemble_stack_op mp op) = assemble_stack_len op"
   by (induction op) simp_all
 
 theorem completesa [simp]: "
   assemble_stack_code cd\<^sub>b \<tturnstile> assemble_state (assembly_map cd\<^sub>b) \<Sigma>\<^sub>u \<leadsto>\<^sub>s\<^sub>a \<Sigma>\<^sub>s\<^sub>a' \<Longrightarrow> 
-    \<exists>\<Sigma>\<^sub>u'. iter (\<tturnstile> assemble_stack_code cd\<^sub>b \<leadsto>\<^sub>s\<^sub>a) \<Sigma>\<^sub>s\<^sub>a' (assemble_state (assembly_map cd\<^sub>b) \<Sigma>\<^sub>u') \<and> 
+    \<exists>\<Sigma>\<^sub>s\<^sub>a'' \<Sigma>\<^sub>u'. iter (\<tturnstile> assemble_stack_code cd\<^sub>b \<leadsto>\<^sub>s\<^sub>a) \<Sigma>\<^sub>s\<^sub>a' (assemble_state (assembly_map cd\<^sub>b) \<Sigma>\<^sub>u') \<and> 
       cd\<^sub>b \<tturnstile> \<Sigma>\<^sub>u \<leadsto>\<^sub>u \<Sigma>\<^sub>u'"
 proof (induction "assemble_stack_code cd\<^sub>b" "assemble_state (assembly_map cd\<^sub>b) \<Sigma>\<^sub>u" \<Sigma>\<^sub>s\<^sub>a' 
        rule: evalsa.induct)
@@ -78,24 +83,118 @@ next
 next
   case (evsa_get pc m mem ps acc)
   thus ?case by simp
+next
+  case (evsa_sub pc k mem ps acc)
+  thus ?case by simp
 qed
 
-theorem correctsa [simp]: "cd\<^sub>b \<tturnstile> \<Sigma>\<^sub>u \<leadsto>\<^sub>u \<Sigma>\<^sub>u' \<Longrightarrow> iter (\<tturnstile> assemble_stack_code cd\<^sub>b \<leadsto>\<^sub>s\<^sub>a) 
-  (assemble_state (assembly_map cd\<^sub>b) \<Sigma>\<^sub>u) (assemble_state (assembly_map cd\<^sub>b) \<Sigma>\<^sub>u')"
+lemma [simp]: "cd ! pc = op \<Longrightarrow> pc < length cd \<Longrightarrow> 
+  assembly_map cd (Suc pc) = assemble_stack_len op + assembly_map cd pc"
+proof (induction cd pc rule: assembly_map.induct)
+  case (2 op' cd)
+  thus ?case by (cases cd) simp_all
+qed simp_all
+
+lemma assemble_code_lookup' [simp]: "cd ! pc = op \<Longrightarrow> pc < length cd \<Longrightarrow> 
+  x < assemble_stack_len op \<Longrightarrow> concat (map (assemble_stack_op (assembly_map (cd' @ cd))) cd) ! 
+    (x + assembly_map cd pc) = assemble_stack_op (assembly_map (cd' @ cd)) op ! x"
+proof (induction cd pc arbitrary: cd' rule: assembly_map.induct)
+  case (3 op' cd y)
+  hence "concat (map (assemble_stack_op (assembly_map ((cd' @ [op']) @ cd))) cd) ! 
+    (x + assembly_map cd y) = assemble_stack_op (assembly_map ((cd' @ [op']) @ cd)) op ! x" 
+      by fastforce
+  hence "(assemble_stack_op (assembly_map (cd' @ op' # cd)) op' @ 
+    concat (map (assemble_stack_op (assembly_map (cd' @ op' # cd))) cd)) !
+      (assemble_stack_len op' + x + assembly_map cd y) =
+        assemble_stack_op (assembly_map (cd' @ op' # cd)) op ! x" by (simp add: nth_append)
+  hence "(assemble_stack_op (assembly_map (cd' @ op' # cd)) op' @ 
+    concat (map (assemble_stack_op (assembly_map (cd' @ op' # cd))) cd)) !
+      (x + (assemble_stack_len op' + assembly_map cd y)) =
+        assemble_stack_op (assembly_map (cd' @ op' # cd)) op ! x" by (metis add.assoc add.commute)
+  thus ?case by simp
+qed (simp_all add: nth_append)
+
+lemma assemble_code_lookup [simp]: "cd ! pc = op \<Longrightarrow> pc < length cd \<Longrightarrow> 
+  x < assemble_stack_len op \<Longrightarrow> 
+    assemble_stack_code cd ! (x + assembly_map cd pc) = assemble_stack_op (assembly_map cd) op ! x"
+  by (metis assemble_code_lookup' append_Nil assemble_stack_code_def)
+
+lemma [simp]: "cd ! pc = op \<Longrightarrow> pc < length cd \<Longrightarrow> 1 < assemble_stack_len op \<Longrightarrow> 
+    assemble_stack_code cd ! (Suc (assembly_map cd pc)) = assemble_stack_op (assembly_map cd) op ! 1"
+  using assemble_code_lookup by fastforce
+
+lemma [simp]: "cd ! pc = op \<Longrightarrow> pc < length cd \<Longrightarrow> 0 < assemble_stack_len op \<Longrightarrow> 
+    assemble_stack_code cd ! (assembly_map cd pc) = assemble_stack_op (assembly_map cd) op ! 0"
+  using assemble_code_lookup by fastforce
+
+lemma [simp]: "m Hp = h \<Longrightarrow> m Env = e \<Longrightarrow> m Vals = vs \<Longrightarrow> m Stk = sh \<Longrightarrow> m = case_memory h e vs sh" 
+  by rule (simp split: memory.splits)
+
+theorem correctsa [simp]: "cd\<^sub>b \<tturnstile> \<Sigma>\<^sub>u \<leadsto>\<^sub>u \<Sigma>\<^sub>u' \<Longrightarrow> restructurable \<Sigma>\<^sub>u cd\<^sub>b \<Longrightarrow> 
+  iter (\<tturnstile> assemble_stack_code cd\<^sub>b \<leadsto>\<^sub>s\<^sub>a) (assemble_state (assembly_map cd\<^sub>b) \<Sigma>\<^sub>u) 
+    (assemble_state (assembly_map cd\<^sub>b) \<Sigma>\<^sub>u')"
 proof (induction cd\<^sub>b \<Sigma>\<^sub>u \<Sigma>\<^sub>u' rule: evalu.induct)
 case (evu_lookup cd pc x e sh sp y h hp ep vs vp)
   then show ?case by simp
 next
   case (evu_pushcon cd pc k h hp e ep vs vp sh sp)
-  from evu_pushcon have "cd ! pc = BPushCon k" by simp
-
-
-  have "iter (\<tturnstile> assemble_stack_code cd \<leadsto>\<^sub>s\<^sub>a)
-     (SAS (\<lambda>m. case m of Hp \<Rightarrow> h | Env \<Rightarrow> e | Vals \<Rightarrow> vs | Stk \<Rightarrow> sh) (\<lambda>m. case m of Hp \<Rightarrow> hp | Env \<Rightarrow> ep | Vals \<Rightarrow> vp | Stk \<Rightarrow> sp)
-       (SOME x. True) (assembly_map cd (Suc pc)))
-     (SAS (\<lambda>m. case m of Hp \<Rightarrow> h(hp := 0, Suc hp := k, Suc (Suc hp) := 0) | Env \<Rightarrow> e | Vals \<Rightarrow> vs(vp := hp) | Stk \<Rightarrow> sh)
-       (\<lambda>m. case m of Hp \<Rightarrow> 3 + hp | Env \<Rightarrow> ep | Vals \<Rightarrow> Suc vp | Stk \<Rightarrow> sp) (SOME x. True) (assembly_map cd pc))" by simp
-  thus ?case by simp
+  let ?mem = "case_memory h e vs sh"
+  let ?ps = "case_memory hp ep vp sp"
+  from evu_pushcon have "assemble_stack_code cd ! (5 + assembly_map cd pc) = SAMov (Mem Hp)" by simp
+  hence "assemble_stack_code cd ! (Suc (Suc (Suc (Suc (Suc (assembly_map cd pc)))))) = 
+    SAMov (Mem Hp)" by (simp add: numeral_def)
+  hence A: "assemble_stack_code cd \<tturnstile> 
+    SAS ?mem ?ps 0 (Suc (Suc (Suc (Suc (Suc (Suc (assembly_map cd pc))))))) \<leadsto>\<^sub>s\<^sub>a 
+      SAS ?mem ?ps hp (Suc (Suc (Suc (Suc (Suc (assembly_map cd pc))))))" 
+    by (metis evsa_mov get_mval.simps(1) memory.simps(13))
+  from evu_pushcon have "assemble_stack_code cd ! (4 + assembly_map cd pc) = SAPush Vals Acc" 
+    by simp
+  hence "assemble_stack_code cd ! (Suc (Suc (Suc (Suc (assembly_map cd pc))))) = SAPush Vals Acc" 
+    by (simp add: numeral_def)
+  hence B: "
+    assemble_stack_code cd \<tturnstile> SAS ?mem ?ps hp (Suc (Suc (Suc (Suc (Suc (assembly_map cd pc)))))) \<leadsto>\<^sub>s\<^sub>a
+      SAS (mem_upd ?mem Vals vp hp) (?ps(Vals := Suc vp)) hp 
+        (Suc (Suc (Suc (Suc (assembly_map cd pc)))))"
+    by (metis evsa_push memory.simps(15) get_val.simps(1))
+  from evu_pushcon have "assemble_stack_code cd ! (3 + assembly_map cd pc) = SAPush Hp (Con 0)" 
+    by simp
+  hence "assemble_stack_code cd ! (Suc (Suc (Suc (assembly_map cd pc)))) = SAPush Hp (Con 0)" 
+    by (simp add: numeral_def)
+  hence C: "assemble_stack_code cd \<tturnstile> SAS (mem_upd ?mem Vals vp hp) (?ps(Vals := Suc vp)) hp 
+    (Suc (Suc (Suc (Suc (assembly_map cd pc))))) \<leadsto>\<^sub>s\<^sub>a SAS (mem_upd (mem_upd ?mem Vals vp hp) Hp hp 0) 
+      (?ps(Vals := Suc vp, Hp := Suc hp)) hp (Suc (Suc (Suc (assembly_map cd pc))))" 
+    by (metis evsa_push get_val.simps(2) fun_upd_apply memory.distinct(3) memory.simps(13))
+  from evu_pushcon have "assemble_stack_code cd ! (2 + assembly_map cd pc) = 
+    SAPush Hp (Con k)" by (simp del: add_2_eq_Suc)
+  hence "assemble_stack_code cd ! (Suc (Suc (assembly_map cd pc))) = SAPush Hp (Con k)" by simp
+  hence D: "assemble_stack_code cd \<tturnstile> SAS (mem_upd (mem_upd ?mem Vals vp hp) Hp hp 0) 
+    (?ps(Vals := Suc vp, Hp := Suc hp)) hp (Suc (Suc (Suc (assembly_map cd pc)))) \<leadsto>\<^sub>s\<^sub>a 
+      SAS (mem_upd (mem_upd (mem_upd ?mem Vals vp hp) Hp hp 0) Hp (Suc hp) k) 
+        (?ps(Vals := Suc vp, Hp := Suc (Suc hp))) hp (Suc (Suc (assembly_map cd pc)))" 
+    by (metis evsa_push get_val.simps(2) fun_upd_apply fun_upd_upd)
+  from evu_pushcon have "assemble_stack_code cd ! Suc (assembly_map cd pc) = SAPush Hp (Con 0)" 
+    by simp
+  hence E: "assemble_stack_code cd \<tturnstile> SAS (mem_upd (mem_upd (mem_upd ?mem Vals vp hp) Hp hp 0) Hp 
+    (Suc hp) k) (?ps(Vals := Suc vp, Hp := Suc (Suc hp))) hp (Suc (Suc (assembly_map cd pc))) \<leadsto>\<^sub>s\<^sub>a
+      SAS (mem_upd (mem_upd (mem_upd (mem_upd ?mem Vals vp hp) Hp hp 0) Hp (Suc hp) k) Hp 
+        (Suc (Suc hp)) 0) (?ps(Vals := Suc vp, Hp := Suc (Suc (Suc hp)))) hp 
+          (Suc (assembly_map cd pc))" 
+    by (metis evsa_push get_val.simps(2) fun_upd_apply fun_upd_upd)
+  from evu_pushcon have "assemble_stack_code cd ! assembly_map cd pc = SAMov (MCon 0)" by simp
+  hence "assemble_stack_code cd \<tturnstile> SAS 
+    (mem_upd (mem_upd (mem_upd (mem_upd ?mem Vals vp hp) Hp hp 0) Hp (Suc hp) k) Hp 
+      (Suc (Suc hp)) 0) (?ps(Vals := Suc vp, Hp := Suc (Suc (Suc hp)))) hp 
+        (Suc (assembly_map cd pc)) \<leadsto>\<^sub>s\<^sub>a SAS 
+          (mem_upd (mem_upd (mem_upd (mem_upd ?mem Vals vp hp) Hp hp 0) Hp (Suc hp) k) Hp 
+            (Suc (Suc hp)) 0) (?ps(Vals := Suc vp, Hp := Suc (Suc (Suc hp)))) 0 
+              (assembly_map cd pc)" 
+    by (metis evsa_mov get_mval.simps(2))
+  with A B C D E have "iter (\<tturnstile> assemble_stack_code cd \<leadsto>\<^sub>s\<^sub>a) 
+    (SAS ?mem ?ps 0 (Suc (Suc (Suc (Suc (Suc (Suc (assembly_map cd pc))))))))
+      (SAS (mem_upd (mem_upd (mem_upd (mem_upd ?mem Vals vp hp) Hp hp 0) Hp (Suc hp) k) Hp 
+        (Suc (Suc hp)) 0) (?ps(Vals := Suc vp, Hp := Suc (Suc (Suc hp)))) 0 (assembly_map cd pc))"
+    by simp
+  with evu_pushcon show ?case by (simp add: numeral_def)
 next
   case (evu_pushlam cd pc pc' h hp e ep vs vp sh sp)
   then show ?case by simp
@@ -113,9 +212,9 @@ next
   then show ?case by simp
 qed
 
-theorem correctsa_iter [simp]: "iter (\<tturnstile> cd\<^sub>b \<leadsto>\<^sub>u) \<Sigma>\<^sub>u \<Sigma>\<^sub>u' \<Longrightarrow> 
-  assemble_stack_code cd\<^sub>b = (cd\<^sub>s\<^sub>a, mp) \<Longrightarrow> 
-    iter (\<tturnstile> cd\<^sub>s\<^sub>a \<leadsto>\<^sub>s\<^sub>a) (assemble_state mp \<Sigma>\<^sub>u) (assemble_state mp \<Sigma>\<^sub>u')"
-  by (induction \<Sigma>\<^sub>u \<Sigma>\<^sub>u' rule: iter.induct) (force, metis correctsa iter_append)
+theorem correctsa_iter [simp]: "iter (\<tturnstile> cd\<^sub>b \<leadsto>\<^sub>u) \<Sigma>\<^sub>u \<Sigma>\<^sub>u' \<Longrightarrow> restructurable \<Sigma>\<^sub>u cd\<^sub>b \<Longrightarrow> 
+  iter (\<tturnstile> assemble_stack_code cd\<^sub>b \<leadsto>\<^sub>s\<^sub>a) 
+    (assemble_state (assembly_map cd\<^sub>b) \<Sigma>\<^sub>u) (assemble_state (assembly_map cd\<^sub>b) \<Sigma>\<^sub>u')"
+  by (induction \<Sigma>\<^sub>u \<Sigma>\<^sub>u' rule: iter.induct) (force, metis correctsa iter_append preserve_restructure)
 
 end
