13StackAssembly/StackAssembly.thy
@@ -5,6 +5,7 @@ begin
 datatype memory = Hp | Env | Vals | Stk
 
 datatype pseudoreg = Acc | Con nat
+datatype pseudomem = Mem memory | MCon nat
 
 datatype sassm_code = 
   BLookup nat
@@ -14,8 +15,9 @@ datatype sassm_code =
 
   | SAPush memory pseudoreg
   | SAPop memory
-  | SAMov memory
+  | SAMov pseudomem
   | SAGet memory
+  | SASub nat
 
 datatype sassm_state = 
   SAS "memory \<Rightarrow> nat \<Rightarrow> nat" "memory \<Rightarrow> nat" nat nat
@@ -30,6 +32,10 @@ primrec get_val :: "pseudoreg \<Rightarrow> nat \<Rightarrow> nat" where
   "get_val Acc x = x"
 | "get_val (Con k) x = k"
 
+primrec get_mval :: "pseudomem \<Rightarrow> (memory \<Rightarrow> nat) \<Rightarrow> nat" where
+  "get_mval (Mem m) x = x m"
+| "get_mval (MCon k) x = k"
+
 fun mem_upd :: "(memory \<Rightarrow> nat \<Rightarrow> nat) \<Rightarrow> memory \<Rightarrow> nat \<Rightarrow> nat \<Rightarrow> memory \<Rightarrow> nat \<Rightarrow> nat" where
   "mem_upd mem m mp k m' x = (if m = m' \<and> mp = x then k else mem m' x)"
 
@@ -41,9 +47,11 @@ inductive evalsa :: "sassm_code list \<Rightarrow> sassm_state \<Rightarrow> sas
 | evsa_pop [simp]: "cd ! pc = SAPop m \<Longrightarrow> ps m = Suc p \<Longrightarrow>
     cd \<tturnstile> SAS mem ps acc (Suc pc) \<leadsto>\<^sub>s\<^sub>a SAS mem (ps(m := p)) (mem m p) pc"
 | evsa_mov [simp]: "cd ! pc = SAMov m \<Longrightarrow>
-    cd \<tturnstile> SAS mem ps acc (Suc pc) \<leadsto>\<^sub>s\<^sub>a SAS mem ps (ps m) pc"
+    cd \<tturnstile> SAS mem ps acc (Suc pc) \<leadsto>\<^sub>s\<^sub>a SAS mem ps (get_mval m ps) pc"
 | evsa_get [simp]: "cd ! pc = SAGet m \<Longrightarrow>
     cd \<tturnstile> SAS mem ps acc (Suc pc) \<leadsto>\<^sub>s\<^sub>a SAS mem ps (mem m acc) pc"
+| evsa_sub [simp]: "cd ! pc = SASub k \<Longrightarrow>
+    cd \<tturnstile> SAS mem ps acc (Suc pc) \<leadsto>\<^sub>s\<^sub>a SAS mem ps (acc - k) pc"
 
 theorem determinismu: "cd \<tturnstile> \<Sigma> \<leadsto>\<^sub>s\<^sub>a \<Sigma>' \<Longrightarrow> cd \<tturnstile> \<Sigma> \<leadsto>\<^sub>s\<^sub>a \<Sigma>'' \<Longrightarrow> \<Sigma>' = \<Sigma>''"
 proof (induction cd \<Sigma> \<Sigma>' rule: evalsa.induct)
@@ -62,6 +70,34 @@ next
   case (evsa_get cd pc m mem ps acc)
   from evsa_get(2, 1) show ?case 
     by (induction cd "SAS mem ps acc (Suc pc)" \<Sigma>'' rule: evalsa.induct) simp_all
+next
+  case (evsa_sub cd pc k mem ps acc)
+  from evsa_sub(2, 1) show ?case 
+    by (induction cd "SAS mem ps acc (Suc pc)" \<Sigma>'' rule: evalsa.induct) simp_all
 qed
+
+lemma [simp]: "mem_upd (case_memory h e vs sh) Hp x y = case_memory (h(x := y)) e vs sh"
+  by (rule+) (simp split: memory.splits)
+
+lemma [simp]: "mem_upd (case_memory h e vs sh) Env x y = case_memory h (e(x := y)) vs sh"
+  by (rule+) (simp split: memory.splits)
+
+lemma [simp]: "mem_upd (case_memory h e vs sh) Vals x y = case_memory h e (vs(x := y)) sh"
+  by (rule+) (simp split: memory.splits)
+
+lemma [simp]: "mem_upd (case_memory h e vs sh) Stk x y = case_memory h e vs (sh(x := y))"
+  by (rule+) (simp split: memory.splits)
+
+lemma [simp]: "(case_memory hp ep vp sp)(Hp := x) = case_memory x ep vp sp"
+  by rule (simp split: memory.splits)
+
+lemma [simp]: "(case_memory hp ep vp sp)(Env := x) = case_memory hp x vp sp"
+  by rule (simp split: memory.splits)
+
+lemma [simp]: "(case_memory hp ep vp sp)(Vals := x) = case_memory hp ep x sp"
+  by rule (simp split: memory.splits)
+
+lemma [simp]: "(case_memory hp ep vp sp)(Stk := x) = case_memory hp ep vp x"
+  by rule (simp split: memory.splits)
 
 end
